pcuic/theories/PCUICPosition.v
@@ -6,7 +6,7 @@ From MetaCoq.Template Require Import config Universes monad_utils utils BasicAst
      AstUtils UnivSubst.
 From MetaCoq.PCUIC Require Import PCUICAst PCUICAstUtils PCUICInduction
      PCUICReflect PCUICLiftSubst PCUICUnivSubst PCUICTyping PCUICCumulativity
-     PCUICSR PCUICReduction.
+     PCUICReduction.
 From Equations Require Import Equations.
 
 Require Import Equations.Prop.DepElim.
